code/experimental/ed25519/Ed25519.fsti
@@ -1,0 +1,24 @@
+module Ed25519
+
+open FStar.Buffer
+
+let uint8_p = buffer UInt8.t
+let hint8_p = buffer Hacl.UInt8.t
+
+val sign:
+  signature:hint8_p{length signature = 64} ->
+  secret:hint8_p{length secret = 32} ->
+  msg:hint8_p ->
+  len:UInt32.t{UInt32.v len = length msg} ->
+  Stack unit
+    (requires (fun h -> live h signature /\ live h msg /\ live h secret))
+    (ensures (fun h0 _ h1 -> live h0 secret /\ live h0 secret /\ live h1 signature /\ modifies_1 signature h0 h1))
+
+val verify:
+  public:uint8_p{length public = 32} ->
+  msg:uint8_p ->
+  len:UInt32.t{length msg = UInt32.v len} ->
+  signature:uint8_p{length signature = 64} ->
+  Stack bool
+    (requires (fun h -> live h public /\ live h msg /\ live h signature))
+    (ensures (fun h0 _ h1 -> modifies_0 h0 h1 /\ live h0 msg /\ live h0 public /\ live h0 signature))
